
\begin{equation*}
  \begin{aligned}
  S \rightarrow & S + S & (1) \\
  S \rightarrow & SS & (2) \\
  S \rightarrow & (S) & (3) \\
  S \rightarrow & S* & (4) \\
  S \rightarrow & a & (5)
\end{aligned}
\end{equation*}

a)

leftmost analysis of $(a + a)*a$:

\begin{equation*}
  \begin{aligned}
          & ((a + a)*a&, &S&, &\epsilon &) \\
 \vdash   & ((a + a)*a&,  &SS&, &2 &) \\
 \vdash   & ((a + a)*a&,  & S*S&, &24&) \\
 \vdash   & ((a + a)*a&,  & (S)*S&, &243&) \\
 \vdash   & (a + a)*a&,  & S)*S&, &243&) \\
 \vdash   & (a + a)*a&,  & S + S)*S&, &2431&) \\
 \vdash   & (a + a)*a&,  & a + S)*S&, &24315&) \\
 \vdash   & (+ a)*a&,  & + S)*S&, &24315&) \\
 \vdash   & (a)*a&,  & S)*S&, &24315&) \\
 \vdash   & (a)*a&,  & a)*S&, &243155&) \\
 \vdash   & ()*a&,  & )*S&, &243155&) \\
 \vdash   & (*a&,  & *S&, &243155&) \\
 \vdash   & (a&,  & S&, &243155&) \\
 \vdash   & (a&,  & a&, &2431555&) \\
 \vdash   & (\epsilon&,  & \epsilon&, &2431555&) \\
\end{aligned}
\end{equation*}

b)

rightmost analysis of $(a + a)*a$:

\begin{equation*}
  \begin{aligned}
          & ((a + a)*a&, &S&, &\epsilon &) \\
 \vdash   & ((a + a)*a&,  &SS&, &2 &) \\
 \vdash   & ((a + a)*a&,  &Sa&, &25 &) \\
 \vdash   & ((a + a)*&,  &S&, &25 &) \\
 \vdash   & ((a + a)*&,  &S*&, &254 &) \\
 \vdash   & ((a + a)&,  &S&, &254 &) \\
 \vdash   & ((a + a)&,  &(S)&, &2543 &) \\
 \vdash   & ((a + a&,  &(S&, &2543 &) \\
 \vdash   & ((a + a&,  &(S+S&, &25431 &) \\
 \vdash   & ((a + a&,  &(S+a&, &254315 &) \\
 \vdash   & ((a +&,  &(S+&, &254315 &) \\
 \vdash   & ((a&,  &(S&, &254315 &) \\
 \vdash   & ((a&,  &(a&, &2543155 &) \\
 \vdash   & ((&,  &(&, &2543155 &) \\
 \vdash   & (\epsilon&,  & \epsilon&, &2543155&) \\
\end{aligned}
\end{equation*}

c) G is not unambiguous. Given the word $aaa$, two possible Syntax trees exist:

\begin{center}
\begin{tikzpicture}[align=center,node distance=10mm,on grid,auto]
   %Syntax:
   %\node[align=<alignment>] (<name>) [<location>] {<text>};
   \node[align=center] (S) []  {S};
   \node[align=center] (temp) [below=of S]  {};
   \node[align=center] (Sa) [left=of temp]  {S};
   \node[align=center] (Sb) [right=of temp]  {S};
   \node[align=center] (Sc) [below=of Sa]  {a};
   \node[align=center] (tempa) [below=of Sb]  {};
   \node[align=center] (Sd) [right=of tempa]  {S};
   \node[align=center] (Se) [left=of tempa]  {S};
   \node[align=center] (Sf) [below=of Sd]  {a};
   \node[align=center] (Sg) [below=of Se]  {a};
   
   %Syntax:
   %\path[<line type>]
   % (<name of start>) edge [<textlocation>, <curve type>] {<text>} (<name of target>)
   \path[->]
    (S) edge (Sa)
        edge (Sb)
    (Sa) edge (Sc)
    (Sb) edge (Sd)
    	 edge (Se)
    (Sd) edge (Sf)
    (Se) edge (Sg);
\end{tikzpicture}
\hspace{20mm}
\begin{tikzpicture}[align=center,node distance=10mm,on grid,auto]
   %Syntax:
   %\node[align=<alignment>] (<name>) [<location>] {<text>};
   \node[align=center] (S) []  {S};
   \node[align=center] (temp) [below=of S]  {};
   \node[align=center] (Sa) [right=of temp]  {S};
   \node[align=center] (Sb) [left=of temp]  {S};
   \node[align=center] (Sc) [below=of Sa]  {a};
   \node[align=center] (tempa) [below=of Sb]  {};
   \node[align=center] (Sd) [right=of tempa]  {S};
   \node[align=center] (Se) [left=of tempa]  {S};
   \node[align=center] (Sf) [below=of Sd]  {a};
   \node[align=center] (Sg) [below=of Se]  {a};
   
   %Syntax:
   %\path[<line type>]
   % (<name of start>) edge [<textlocation>, <curve type>] {<text>} (<name of target>)
   \path[->]
    (S) edge (Sa)
        edge (Sb)
    (Sa) edge (Sc)
    (Sb) edge (Sd)
    	 edge (Se)
    (Sd) edge (Sf)
    (Se) edge (Sg);
\end{tikzpicture}
\end{center}

because the derivation $S \rightarrow SS | a$ is part of $G$. Since two different derivations exist, $G$ cannot be unambiguous.