\subsection*{a)}

To extend the statement of Theorem 6.10, we first define $la_k(\pi)$ with $\pi := A \rightarrow \beta \in P$ as follows:
\begin{equation*}\begin{split}
la_k(\pi) := first_k(\beta \cdot follow_k(A)) \subseteq \Sigma_{\epsilon}^*
\end{split}\end{equation*}

Then $G$ is in $LL(k)$ for arbitrary $k \in \mathbb{N}_0 \Leftrightarrow la_k(A \rightarrow \beta) \cap la_k(A \rightarrow \gamma) = \emptyset$ for all pairs of rules $A \rightarrow \beta | \gamma \in P$ with $\beta \neq \gamma$.

\subsection*{b)}

\subsubsection*{First characterization:}

Iterate over all possible derivations \begin{equation*}
S \Rightarrow_l^{*} wA\alpha \begin{cases}\Rightarrow_l w\beta\alpha\\ \Rightarrow_l w\gamma\alpha\end{cases}
\end{equation*} and test if \begin{equation*}
first_1(\beta\alpha) \cap first_1(\gamma\alpha) = \emptyset
\end{equation*}

\textbf{1.}
\begin{equation*}
\begin{split}
S \Rightarrow_l^{0} \epsilon S\epsilon \begin{cases}\Rightarrow_l \epsilon aAab\epsilon\\ \Rightarrow_l \epsilon bAbb\epsilon\end{cases} \\
first_2(aAab\epsilon) = \{aa\} \\
first_2(bAbb\epsilon) = \{ba, bb\} \\
\{aa\} \cap \{ba, bb\} = \emptyset \quad \checkmark
\end{split}
\end{equation*}

\textbf{2.}
\begin{equation*}
\begin{split}
S \Rightarrow_l^{1} aAab \begin{cases}\Rightarrow_l aaab\\ \Rightarrow_l \epsilon a\epsilon ab\end{cases} \\
first_2(aab) = \{aa\} \\
first_2(\epsilon ab) = \{ab\} \\
\{aa\} \cap \{ab\} = \emptyset \quad \checkmark
\end{split}
\end{equation*}

\textbf{3.}
\begin{equation*}
\begin{split}
S \Rightarrow_l^{1} bAbb \begin{cases}\Rightarrow_l babb\\ \Rightarrow_l \epsilon b\epsilon bb\end{cases} \\
first_2(abb) = \{ab\} \\
first_2(\epsilon bb) = \{bb\} \\
\{ab\} \cap \{bb\} = \emptyset \quad \checkmark
\end{split}
\end{equation*}

Thus $G \in LL(2)$.

\subsubsection*{Second characterization:}

For all pairs of rules $A \rightarrow \beta | \gamma \in P, \beta \neq \gamma$, check if
\begin{equation*}
la_2(A\rightarrow \beta) \cap la_2(A\rightarrow \gamma) = \emptyset
\end{equation*}

\textbf{1.} $S \rightarrow aAab | bAbb$:
\begin{equation*}
\begin{split}
follow_2(S) = \{\epsilon\} \\
la_2(S\rightarrow aAab) = first_2(aAab \cdot \{\epsilon\}) = \{aa\} \\
la_2(S\rightarrow bAbb) = first_2(bAbb \cdot \{\epsilon\}) = \{ba, bb\} \\
\{aa\} \cap \{ba, bb\} = \emptyset \quad \checkmark
\end{split}
\end{equation*}

\textbf{2.} $A \rightarrow a | \epsilon$:
\begin{equation*}
\begin{split}
follow_2(A) = \{ab, bb\} \\
la_2(A\rightarrow a) = first_2(a \cdot \{ab, bb\}) = \{aa, ab\} \\
la_2(A\rightarrow \epsilon) = first_2(\epsilon \cdot \{ab, bb\}) = \{ab, bb\} \\
\{aa, ab\} \cap \{ab, bb\} \neq \emptyset \quad \text{\Lightning}
\end{split}
\end{equation*}

Thus (incorrectly) $G \not\in LL(2)$.