\subsection*{a)}

Using Theorem 6.10, check $la(L \rightarrow S)$ and $la(S \rightarrow SS)$:

\begin{equation*}
\begin{split}
la(L \rightarrow S) = fi(S \cdot fo(L)) = fi(S \cdot \{), ,\}) = \{(, a\} \\
la(L \rightarrow SS) = fi(SS \cdot fo(L)) = fi(SS \cdot \{), ,\}) = \{(, a \} \\
\{(, a\} \cap \{(, a\} = \{(, a\}
\end{split}
\end{equation*}

Thus, $G \not\in LL(1)$.

\subsection*{b)}

\begin{equation*}
\begin{split}
&S \rightarrow (L) | a \\
&L \rightarrow L,S | L,SS | S | SS
\end{split}
\end{equation*}

First step: remove left recursion

\begin{equation*}
\begin{split}
&S \rightarrow (L) | a \\
&L \rightarrow SL^{'} | SSL^{'} \\
&L^{'} \rightarrow \epsilon | ,SL^{'} | ,SSL^{'}
\end{split}
\end{equation*}

Second step: left factorization

\begin{equation*}
\begin{split}
&S \rightarrow (L) | a \\
&L \rightarrow SL^{''} \\
&L^{''} \rightarrow L^{'} | SL^{'} \\
&L^{'} \rightarrow \epsilon | ,SL^{''}
\end{split}
\end{equation*}

\subsection*{c)}

Prove using Theorem 6.10:

\textbf{1.} $S \rightarrow (L) | a$:
\begin{equation*}
\begin{split}
fo(S) = \{(, a, ), \epsilon, ,\} \\
la(S \rightarrow (L)) = fi((L) \cdot fo(S)) = \{ ( \} \\
la(S \rightarrow a) = fi(a \cdot fo(S)) = \{ a \} \\
\{ ( \} \cap \{ a \} = \emptyset \quad \checkmark
\end{split}
\end{equation*}

\textbf{2.} $L^{''} \rightarrow L^{'} | SL^{'}$:
\begin{equation*}
\begin{split}
fo(L^{''}) = \{)\} \\
la(L^{''} \rightarrow L^{'}) = fi(L^{'} \cdot fo(L^{''})) = \{ ), , \} \\
la(L^{''} \rightarrow SL^{'}) = fi(SL^{'} \cdot fo(L^{''})) = \{ (, a \} \\
\{ ), , \} \cap \{ (, a \} = \emptyset \quad \checkmark
\end{split}
\end{equation*}

\textbf{3.} $L^{'} \rightarrow \epsilon | ,SL^{''}$:
\begin{equation*}
\begin{split}
fo(L^{'}) = \{)\} \\
la(L^{'} \rightarrow \epsilon) = fi(\epsilon \cdot fo(L^{'})) = \{ ) \} \\
la(L^{'} \rightarrow ,SL^{''}) = fi(,SL^{''} \cdot fo(L^{'})) = \{ , \} \\
\{ ) \} \cap \{ , \} = \emptyset \quad \checkmark
\end{split}
\end{equation*}

Thus $G' \in LL(1)$.