Grammar (Start symbol $S$):

\begin{equation*}
\begin{aligned}
S & \rightarrow E & Val.0 &=  Val.1 \\
E & \rightarrow F & Val.0 &=  Val.1 \\
E & \rightarrow E + F & Val.0 &=  Val.1 + Val.3 \\
F & \rightarrow T & Val.0 &=  Val.1 \\
F & \rightarrow F * T & Val.0 &=  Val.1 * Val.3 \\
T & \rightarrow N & Val.0 &=  Val.1 \\
T & \rightarrow (E) & Val.0 &=  Val.1 \\
N & \rightarrow N D & Val.0 &=  Val.1 * 10 + Val.2 \\
N & \rightarrow D & Val.0 &=  Val.1 \\
D & \rightarrow 0 & Val.0 &=  0 \\
D & \rightarrow 1 & Val.0 &=  1 \\
D & \rightarrow 2 & Val.0 &=  2 \\
D & \rightarrow 3 & Val.0 &=  3 \\
D & \rightarrow 4 & Val.0 &=  4 \\
D & \rightarrow 5 & Val.0 &=  5 \\
D & \rightarrow 6 & Val.0 &=  6 \\
D & \rightarrow 7 & Val.0 &=  7 \\
D & \rightarrow 8 & Val.0 &=  8 \\
D & \rightarrow 9 & Val.0 &=  9 
\end{aligned}
\end{equation*}

Parse tree for $2 * 5 + 3$:

\begin{center}
\begin{tikzpicture}[align=center,node distance=12mm,on grid,auto]
   %Syntax:
   %\node[align=<alignment>] (<name>) [<location>] {<text>};
   \node[align=center] (S) []  {$k_0$ : S};
   \node[align=center] (E) [below=of S]  {$k_1$ : E};
   \node[align=center] (E+F2) [below=of E]  {$k_{14}$ : +};
   \node[align=center] (E+F1) [left=2cm of E+F2]  {$k_2$ : E};
   \node[align=center] (E+F3) [right=2cm of E+F2]  {$k_{15}$ : F};
   \node[align=center] (F+T1) [below=of E+F1]  {$k_3$ : F};
   \node[align=center] (F+T2) [below=of E+F3]  {$k_{16}$ : T};
   \node[align=center] (F*T+N2) [below=of F+T1]  {$k_9$ : *};
   \node[align=center] (F*T+N1) [left=2cm of F*T+N2]  {$k_4$ : F};
   \node[align=center] (F*T+N3) [right=2cm of F*T+N2]  {$k_{10}$ : T};
   \node[align=center] (F*T+N4) [below=of F+T2]  {$k_{17}$ : N};
   \node[align=center] (T*N+D1) [below=of F*T+N1]  {$k_5$ : T};
   \node[align=center] (T*N+D2) [below=of F*T+N3]  {$k_{11}$ : N};
   \node[align=center] (T*N+D3) [below=of F*T+N4]  {$k_{18}$ : D};
   \node[align=center] (N*D+31) [below=of T*N+D1]  {$k_6$ : N};
   \node[align=center] (N*D+32) [below=of T*N+D2]  {$k_{12}$ : D};
   \node[align=center] (N*D+33) [below=of T*N+D3]  {$k_{19}$ : 3};
   \node[align=center] (D*5+31) [below=of N*D+31]  {$k_7$ : D};
   \node[align=center] (D*5+32) [below=of N*D+32]  {$k_{13}$ : 5};
   \node[align=center] (2*5+3) [below=of D*5+31]  {$k_8$ : 2};
   
   %Syntax:
   %\path[<line type>]
   % (<name of start>) edge [<textlocation>, <curve type>] {<text>} (<name of target>)
    \path[-]
      (S) edge (E)
      (E) edge (E+F1)
          edge (E+F2)
          edge (E+F3)
      (E+F1) edge (F+T1)
      (E+F3) edge (F+T2)
      (F+T1) edge (F*T+N1)
             edge (F*T+N2)
             edge (F*T+N3)
      (F+T2) edge (F*T+N4)
      (F*T+N1) edge (T*N+D1)
      (F*T+N3) edge (T*N+D2)
      (F*T+N4) edge (T*N+D3)
      (T*N+D1) edge (N*D+31)
      (T*N+D2) edge (N*D+32)
      (T*N+D3) edge (N*D+33)
      (N*D+31) edge (D*5+31)
      (N*D+32) edge (D*5+32)
      (D*5+31) edge (2*5+3)
      ;
\end{tikzpicture}
\end{center}

\pagebreak

Equation system:

\begin{equation*}
\begin{aligned}
E_{k_0} &: Val.k_0 = Val.k_1 \\
E_{k_1} &: Val.k_1 = Val.k_2 + Val.k_{15} \\
E_{k_2} &: Val.k_2 = Val.k_3 \\
E_{k_3} &: Val.k_3 = Val.k_4 * Val.k_{10} \\
E_{k_4} &: Val.k_4 = Val.k_5 \\
E_{k_5} &: Val.k_5 = Val.k_6 \\
E_{k_6} &: Val.k_6 = Val.k_7 \\
E_{k_7} &: Val.k_7 = 2 \\
E_{k_{10}} &: Val.k_{10} = Val.k_{11} \\
E_{k_{11}} &: Val.k_{11} = Val.k_{12} \\
E_{k_{12}} &: Val.k_{12} = 5 \\
E_{k_{15}} &: Val.k_{15} = Val.k_{16} \\
E_{k_{16}} &: Val.k_{16} = Val.k_{17} \\
E_{k_{17}} &: Val.k_{17} = Val.k_{18} \\
E_{k_{18}} &: Val.k_{18} = 3 \\
\end{aligned}
\end{equation*}

Solution:

\begin{equation*}
\begin{aligned}
E_{k_0} &: Val.k_0 = 13 \\
E_{k_1} &: Val.k_1 = 10 + 3 = 13 \\
E_{k_2} &: Val.k_2 = 10 \\
E_{k_3} &: Val.k_3 = 2 * 5 = 10 \\
E_{k_4} &: Val.k_4 = 2 \\
E_{k_5} &: Val.k_5 = 2 \\
E_{k_6} &: Val.k_6 = 2 \\
E_{k_7} &: Val.k_7 = 2 \\
E_{k_{10}} &: Val.k_{10} = 5 \\
E_{k_{11}} &: Val.k_{11} = 5 \\
E_{k_{12}} &: Val.k_{12} = 5 \\
E_{k_{15}} &: Val.k_{15} = 3 \\
E_{k_{16}} &: Val.k_{16} = 3 \\
E_{k_{17}} &: Val.k_{17} = 3 \\
E_{k_{18}} &: Val.k_{18} = 3 
\end{aligned}
\end{equation*}

Thus $E_t = 13$.